\subsection{Layered models}
General solution approach of eq. 3.13.
\begin{align*}
\frac{d^2\hat{E}_x}{dz^2}=(i\omega\mu_0\sigma+k^2)\hat{E}_x
\end{align*}
in the $\omega,k$ domain for TE-fields $(E_z=0)$ for the m. layer.

\begin{align*}
\hat{E}_x(z)=A_me^{-K_m z}+B_me^{K_m z}&& z_m<z<z_{m+1}
\end{align*}

with 
\begin{align}
K_m=\sqrt{i\omega\mu_0\sigma+k^2}
\end{align}

\begin{align*}
\hat{B}_z=k(Ee^{-kz}-Ie^{kz})
\end{align*}


Using eq. 3.15 ($\hat{B}_y=-\frac{1}{i\omega}\frac{d\hat{E}_x}{dz}$):

\begin{align}
\hat{B}_y=\frac{-1}{i\omega}\frac{d\hat{E}_x}{dz}=\frac{K_m}{i\omega}(A_me^{-K_m z}+B_me^{K_m z})
\end{align}

For the homogeneous half space of the model:

\begin{align*}
\hat{E}_x(z)=A_me^{-K_m z} && \hat{B}_y(z)=\frac{K_m}{i\omega}A_m e^{-K_m z}
\end{align*}

Analogous for $\hat{E}_y$ and $\hat{B}_x$ (see chapter 3.4).

Continuity of $\hat{E}_x$ and $\hat{B}_y$ at the layer boundaries are valid if their impedance ratio:

\begin{align}
\frac{\hat{E}_x}{\hat{B}_y}=\frac{i\omega}{K_mG(z)}
\end{align}

with 
\begin{align}
G(z)=\frac{A_me^{-K_m z}-B_me^{K_m z}}{A_me^{-K_m z}+B_me^{K_m z}}
\end{align}

is continuous. $G(z)$ changes as the ratio of the vertical wave numbers.

\begin{align*}
K_m \underbrace{G_M^+}_{G(z_{m+1}^{-0})}=K_{m+1}\underbrace{G_{m+1}^-}_{G(z_{m+1}^{+0})}
\end{align*}
for $z=z_{m+1}$.
\begin{align*}
G_m^+=\frac{K_{m+1}}{K_m}G_{m+1}^-
\end{align*}
For the half space of the model:
\begin{align*}
G_{m}^-=1
\end{align*} 

For the connection to the air region: $K_0G_0^+=K_1G_1^-$.

For the connection $G_m^-$ to $G_m^+$:
\begin{align}
K_mz_{m+1}=K_mz_m+K_md_m
\label{eq:eq6-5}
\end{align}
with $d_m=z_{m+1}-z_m$ the thickness of the $m$'th layer.

\begin{align*}
\Rightarrow e^{\pm K_mz_{m+1}}=e^{\pm\alpha}\left(\cosh(\beta)\pm\sinh(\beta)\right)
\end{align*}
Now insert in the eq. 3.4 $(G(z) = ...)$ for $z=z_{m+1}^{-0}$

\begin{align}
G_m^+=\frac{(A_me^{-\alpha}-\beta e^\alpha)\cosh(\beta)-(A_me^{-\alpha}+\beta e^\alpha)\sinh(\beta)}{(A_me^{-\alpha}+\beta e^\alpha)\cosh(\beta)-(A_me^{-\alpha}-\beta e^\alpha)\sinh(\beta)}
\end{align}

Divide by $(A_me^{-\alpha}+\beta e^\alpha)\cosh(\beta)$

\begin{align*}
G_m^+=\frac{G_m^--\tanh(\beta)}{1-G_m^-\tanh(\beta)}
\end{align*}
or 
\begin{align*}
G_m^+=\frac{G_m^++\tanh(\beta)}{1+G_m^+\tanh(\beta)}
\end{align*}
Inserting of eq. \eqref{eq:eq6-5} yields the \textit{Recursion formula of WAIT}:

\begin{align}
G_m^-=\frac{K_{m+1}G_{m+1}^-+K_m\tanh(K_md_m)}{K_m+K_{m+1}G_{m+1}^-\tanh(K_md_m)}
\end{align}


Steps to do:
Successive selection for a given ground model. For $m=M-1,M-2,...,2,1$, $G_M^-=1$ and determination of $G_1^-$ for the ground surface at $z=\pm 0$. If $G_1^-$ is determined, calculate impedance $z$ or complex penetration depth $C$ according to
\begin{align*}
\frac{\hat{E}_x}{\hat{E}_y}=\frac{i\omega}{K_mG(z)}
\end{align*}
Then 
\begin{align}
\hat{E}_x(0,k,\omega)=i\omega C(k,\omega)\hat{B}_y(0,k,\omega)
\end{align}
with $C(k,\omega)=(G_1^-K_1)^{-1}$

Extended definition compared to eq. 2.18:

\begin{align*}
C(k,\omega)=K^{-1}=\frac{p}{2}(1-i)
\end{align*}
\begin{align}
C(k,\omega)=\frac{\hat{E}_x(0,k,\omega)}{-\frac{d\hat{E}_x}{dz}\bigg|_{z=0}}=\frac{\hat{E}_x}{i\omega\hat{B}_y}
\end{align}

\newcommand{\Ehat}{\hat{E}}
\newcommand{\Bhat}{\hat{B}}

\subsubsection*{Analogous solution approach for $B_y$ for the induction by TM fields:}
\begin{align*}
\hat{B}_y=a_me^{-K_mz}+b_me^{K_mz}
\end{align*}
Using eq. 2.21:
\begin{align*}
\Ehat=-\frac{1}{\mu_0\sigma}\frac{d\Bhat_y}{dz}
\end{align*}
See chapter 2: solution for the TM fields.
\begin{align*}
\Ehat_x=-\frac{1}{\mu_0\sigma}\frac{d\Bhat_y}{dz}=\frac{K_m}{\mu_0\sigma_m}\left(a_me^{-K_mz}-b_me^{K_mz}\right)
\end{align*}
From the continuity of the impedance (admittance) follows:

\begin{align*}
\frac{\Bhat_y}{\Ehat_x}=\frac{\mu_0\sigma_m}{K_m g(z)}
\end{align*}
with
\begin{equation}
g(z)=\frac{a_me^{-K_mz}+b_me^{K_mz}}{a_me^{-K_mz}-b_me^{K_mz}}
\label{eq:6-10}
\end{equation}
\subsubsection*{Boundary conditions for TM-fields}
\begin{equation}
K_m g_m^+\rho_m=K_{m+1}g_{m+1}^-\rho_{m+1}
\label{eq:6-bc-1}
\end{equation}
$\Rightarrow$
\begin{equation}
g_m^-=\frac{K_{m+1}g_{m+1}^-\rho_{m+1}+K_m\rho_m\tanh(K_md_m)}{K_m\rho_m+K_{m+1}g_{m+1}^-\rho_{m+1}\tanh(K_md_m)}
\label{eq:6-bc-2}
\end{equation}

From \eqref{eq:6-bc-2} we get $g_1^-$ for the ground surface and from \eqref{eq:6-10} the admittance:

\begin{equation*}
\Bhat_y(0,k,\omega)=\mu_0\sigma_1 C(k,\omega)\Ehat_x(0,k,\omega)
\end{equation*}
with $C=(K_1 g_1^-)^{-1}$

We consider quasi-homogeneous TM-source fields: $K_m^2=i\omega\mu_0\sigma_m$ for all layers. 

We divide \eqref{eq:6-bc-2} by $i\omega\mu_0$:

\begin{align*}
\frac{K_mg_m^+}{i\omega\mu_0\sigma_m}=\frac{g_m^+}{K_m}
\end{align*}
and 
\begin{align*}
\frac{K_{m+1}g_{m+1}^-}{i\omega\mu_0\sigma_{m+1}}=\frac{g_{m+1}^-}{K_{m+1}}
\end{align*}
(see eq. \eqref{eq:6-5} with $\frac{1}{g_m^+}=\frac{K_{m+1}}{K_m}\frac{1}{g_{m+1}^-}$)

or
\begin{align*}
\frac{K_m}{g_m^-}=\frac{K_{m+1}}{g_{m+1}^-}
\end{align*}
according to \eqref{eq:6-5} for TE fields with $g(z)=\frac{1}{G(z)}$

The recursion formula of Wait yields the inverse of $g_1^-$:
\begin{align*}
g_1^-=\frac{1}{G_1^-}
\end{align*}
for $k=0$. And the impedance $z$ of quasi-homogeneous fields:
\begin{align*}
\Ehat_x(0,k,\omega)=z(k,\omega)\Bhat_y(0,k,\omega)
\end{align*}
will be
\begin{align*}
z(k,\omega)=\frac{K_1g_1^-}{\mu_0\sigma_1}=\frac{K_1i\omega}{i\omega\mu_0\sigma_1G_1^-}=i\omega C(k,\omega)
\end{align*}

\subsection{Transfer functions for time-dependent fields}

\begin{itemize}
\item $z(k,\omega)\rightarrow$ Impedance
\item $C(k,\omega)\rightarrow$ Complex penetration depth
\item $Q(k,\omega)\rightarrow$ Potential ratio of internal to external part
\end{itemize}
Transfer functions for TE-fields for $z=0$ and $\sigma=\sigma(z)$:

\begin{align*}
\Ehat_x&=z\Bhat_y && \Ehat_y=-z\Bhat_x\\
\Bhat_z&=C(ik_x\Bhat_x+ik_y\Bhat_y) && I=QE\\
\end{align*}
with $z=i\omega C$ and
\begin{equation}
\begin{split}
Q&=\frac{1-kC}{1+kC}\\
C&=\frac{1}{K_1G_1^-}
\end{split}
\end{equation}
\subsubsection*{Examples}
\begin{enumerate}
\item Homogeneous half space with $\sigma = const \Rightarrow G_1^-=1$, $C(k,\omega)=K^{-1}$ with 
\begin{equation}
K^2=i\omega\mu_0\sigma+k^2
\end{equation}

\item 
\begin{figure}
\begin{center}
\resizebox{0.4\textwidth}{!}
{
\begin{pspicture}(0,-1.358125)(5.4009376,1.358125)
\psline[linewidth=0.04cm](1.3809375,1.1596875)(5.3809376,1.1596875)
\psline[linewidth=0.04cm](1.3809375,-0.4403125)(5.3809376,-0.4403125)
\usefont{T1}{ptm}{m}{n}
\rput(0.41234374,1.1646875){$z=0$}
\usefont{T1}{ptm}{m}{n}
\rput(0.53234375,-0.4353125){$h$}
\usefont{T1}{ptm}{m}{n}
\rput(3.1923437,0.6646875){$\sigma=0$}
\usefont{T1}{ptm}{m}{n}
\rput(3.4823437,-1.1353126){$\sigma=\infty$}
\end{pspicture} 
}
\end{center}
\end{figure}
$K_1=k$, $|K_2|=\infty$, $G_1^-=\frac{1}{\tanh(kh)}$, $C(k)=\frac{1}{k}\tanh(kh)$

For $kp \rightarrow 0$, $kh\rightarrow 0$:

\begin{itemize}
\item \underline{1. Model:}
$C(k,\omega)=C_0(k,\omega)=\frac{p}{1+i}$

..........................????????

\item \underline{2. Model:}
$C(k)\rightarrow C_0=h$
For $kp\rightarrow \infty$, $kh\rightarrow\infty$: $C(k,\omega)=1/k$.


\end{itemize}

\begin{figure}[H]
\begin{center}
\resizebox{0.5\textwidth}{!}
{
\begin{pspicture}(0,-3.2784376)(8.342813,3.2584374)
\psline[linewidth=0.04cm,arrowsize=0.05291667cm 2.0,arrowlength=1.4,arrowinset=0.4]{->}(1.6809375,-0.7615625)(1.6809375,3.2384374)
\psline[linewidth=0.04cm,arrowsize=0.05291667cm 2.0,arrowlength=1.4,arrowinset=0.4]{->}(1.6809375,-0.7615625)(7.6809373,-0.7615625)
\psbezier[linewidth=0.04](1.6809375,2.6384375)(6.8809376,2.6384375)(5.3031597,0.6384375)(7.0809374,-0.3615625)
\psbezier[linewidth=0.04,linestyle=dashed,dash=0.16cm 0.16cm](1.6809375,2.5384376)(6.6809373,2.5384376)(5.3031597,0.5384375)(7.0809374,-0.4615625)
\psline[linewidth=0.04cm](3.5809374,2.5384376)(3.5809374,-0.7615625)
\usefont{T1}{ptm}{m}{n}
\rput(1.0423437,2.9434376){$C(k,\omega)$}
\usefont{T1}{ptm}{m}{n}
\rput(8.032344,-1.0565625){$k$}
\psline[linewidth=0.04cm,arrowsize=0.05291667cm 2.0,arrowlength=1.4,arrowinset=0.4]{->}(2.9809375,-2.8615625)(2.7809374,0.2384375)
\usefont{T1}{ptm}{m}{n}
\rput(4.295469,-3.0565624){C does not depend on k}
\end{pspicture} 
}
\caption{$C$ for Model 1}
\label{fig:c-model1}
\end{center}
\end{figure}

\begin{figure}
\begin{center}
\resizebox{0.5\textwidth}{!}
{
\begin{pspicture}(0,-3.2784376)(8.342813,3.2584374)
\psline[linewidth=0.04cm,arrowsize=0.05291667cm 2.0,arrowlength=1.4,arrowinset=0.4]{->}(1.6809375,-0.7615625)(1.6809375,3.2384374)
\psline[linewidth=0.04cm,arrowsize=0.05291667cm 2.0,arrowlength=1.4,arrowinset=0.4]{->}(1.6809375,-0.7615625)(7.6809373,-0.7615625)
\psbezier[linewidth=0.04](3.5809374,2.5384376)(4.5809374,0.4384375)(5.4809375,0.1384375)(7.2809377,-0.4615625)
\psline[linewidth=0.04cm](3.5809374,2.5384376)(3.5809374,-0.7615625)
\usefont{T1}{ptm}{m}{n}
\rput(1.0423437,2.9434376){$C(k,\omega)$}
\usefont{T1}{ptm}{m}{n}
\rput(8.032344,-1.0565625){$k$}
\psline[linewidth=0.04cm,arrowsize=0.05291667cm 2.0,arrowlength=1.4,arrowinset=0.4]{->}(2.9809375,-2.8615625)(2.7809374,0.2384375)
\usefont{T1}{ptm}{m}{n}
\rput(4.295469,-3.0565624){C does not depend on k}
\psline[linewidth=0.04cm](1.6809375,2.5384376)(3.5809374,2.5384376)
\psline[linewidth=0.04cm,arrowsize=0.05291667cm 2.0,arrowlength=1.4,arrowinset=0.4]{->}(5.9809375,1.4384375)(5.2809377,0.5384375)
\usefont{T1}{ptm}{m}{n}
\rput(6.572344,1.7434375){$1/k$}
\end{pspicture} 
}
\caption{$C$ for Model 2}
\label{fig:c-model2}
\end{center}
\end{figure}
\end{enumerate}
Definition of complex penetration depth for quasi-homogeneous-fields:
\begin{align*}
C_0(\omega)=C(0,\omega),~~~~z_0(\omega)=z(0,\omega)
\end{align*}
with $k|C|^2\ll 1$ or $|C_0|^2\ll \lambda$ for all wave numbers of the source field
\begin{align*}
\Ehat_x=z_0\Bhat_y && \Ehat_y=...\\
\Bhat_z=C_0(...) &&with~~ |\Bhat_z|\ll|\Bhat_{xy}|
\end{align*}
This is also valid for TM-fields with admittance $A(k,\omega)$ as transfer function (from eq. 6.13)
\begin{equation}
\begin{split}
\Bhat_x=A(k,\omega)\Ehat_y\\
\Bhat_y=A(k,\omega)\Ehat_x\\
\Ehat_z=C(k,\omega)(ik_x\Ehat_x+ik_y\Ehat_y)
\end{split}
\end{equation}
with $A=\mu_0\sigma C$ and $C=\frac{1}{K_1g_1^-}$ for layered ground.

At all depth ranges $\omega\mu_0\sigma\gg k^2$ and therefore $K_m=\sqrt{i\omega\mu_0\sigma_m}$ and $C=(K_1G_1^-)^{-1}$

\begin{align*}
C_0^{(TE)}=\frac{1}{K_1G_1^-}&& C_0^{(TM)}=\frac{G_1^-}{K_1}
\end{align*}

\begin{equation}
i\omega\mu_0\sigma C_0^{(TE)}C_0^{(TM)}=1
\end{equation}

\subsection{Complex penetration depth $C$ for simple conductivities}

\subsubsection*{Model 1, 2}
!!!!!!!!!!!!!!!!!!!!model 1, mode2 bilder

$C(k,\omega)=K^{-1}\rightarrow\frac{p}{1+i}$

$K_2=\infty$ and 

\begin{equation}
G_1^-=\frac{1}{\tanh(K_1h}
\end{equation}

$C(k,\omega)=\frac{\tanh(K_1h}{K_1}\stackrel{kp\rightarrow 0}\rightarrow\frac{p_1}{1+i}\tanh\left(\frac{(1+i)h}{p_1}\right)$

for $h\ll p_1 \Rightarrow C_0=h \Rightarrow$ compare with eq. 6.18

\subsubsection*{Model 3}

$K_2=k$
For $|K_1|\gg k (\rho k\ll 1) \Rightarrow G_1^-=\tanh(K_1d)$

$C(k,\omega)=\frac{\coth(K_1d}{K_1}$ !!!!!!!!!!!!!!!????????

....
$C_0=\frac{1}{3}d+\frac{p_1^2}{2id}$

\subsubsection*{Representation of $C(\omega)$ with $T=\frac{2\pi}{\omega}$ as a parameter for models 1,2,3}

\begin{figure}[H]
\begin{center}
\resizebox{0.6\textwidth}{!}
{
\begin{pspicture}(0,-3.308125)(11.522813,3.308125)
\psline[linewidth=0.04cm,arrowsize=0.05291667cm 2.0,arrowlength=1.4,arrowinset=0.4]{->}(1.7809376,2.8096876)(1.7809376,-3.1903124)
\psline[linewidth=0.04cm,arrowsize=0.05291667cm 2.0,arrowlength=1.4,arrowinset=0.4]{->}(1.7809376,2.8096876)(9.780937,2.8096876)
\usefont{T1}{ptm}{m}{n}
\rput(10.622344,3.1146874){$-Im(C_0)$}
\usefont{T1}{ptm}{m}{n}
\rput(0.76234376,-3.0853126){$Re(C_0)$}
\psline[linewidth=0.04cm](1.7809376,2.8096876)(9.580937,-1.7903125)
\usefont{T1}{ptm}{m}{n}
\rput(9.855938,-0.9853125){Model 1}
\psline[linewidth=0.04cm,arrowsize=0.05291667cm 2.0,arrowlength=1.4,arrowinset=0.4]{->}(5.1809373,0.6096875)(5.9809375,0.1096875)
\usefont{T1}{ptm}{m}{n}
\rput(6.162344,-0.0853125){$T$}
\psbezier[linewidth=0.04,linestyle=dashed,dash=0.16cm 0.16cm](1.7809376,2.8096876)(4.9809375,1.0096875)(5.5809374,-0.6903125)(1.8809375,-2.1903124)
\usefont{T1}{ptm}{m}{n}
\rput(3.3704689,-2.1853125){Model 2}
\psbezier[linewidth=0.04,linestyle=dashed,dash=0.16cm 0.16cm](1.8809375,2.7096875)(3.6809375,1.6096874)(5.0809374,1.5763541)(8.680938,1.3874652)
\usefont{T1}{ptm}{m}{n}
\rput(8.862968,1.0146875){Model 3}
\end{pspicture} 
}
\caption{Real and Imaginary part of $C$ in dependency of $T$}
\label{fig:crealimag}
\end{center}
\end{figure}

\subsubsection*{Model 4}
\begin{figure}[H]
\begin{center}
\resizebox{0.4\textwidth}{!}
{
\begin{pspicture}(0,-1.008125)(5.0009375,1.008125)
\psline[linewidth=0.04cm](0.9809375,0.8096875)(4.9809375,0.8096875)
\psline[linewidth=0.04cm](0.9809375,-0.1903125)(4.9809375,-0.1903125)
\usefont{T1}{ptm}{m}{n}
\rput(0.41234374,0.8146875){$z=0$}
\usefont{T1}{ptm}{m}{n}
\rput(0.23234375,-0.1853125){$h$}
\usefont{T1}{ptm}{m}{n}
\rput(3.6723437,0.2146875){$\sigma_1=0$}
\usefont{T1}{ptm}{m}{n}
\rput(3.4823437,-0.7853125){$\sigma_2$}
\end{pspicture} 
}
\caption{Model 4}
\label{fig:6-model4}
\end{center}
\end{figure}

$K_1=k$ for $|K_2|\gg k \Rightarrow G_1^-=\frac{K_2}{k+K_2\tanh(kh)}$ and
\begin{align*}
C(k,\omega)=\frac{k+K_2\tanh(kh)}{K_2k}\stackrel{kh\rightarrow 0}\rightarrow=h+\frac{p_2}{1+i}=h+\frac{p_2}{2}-\frac{ip_2}{2}
\end{align*}

\subsubsection*{Model 5}
\begin{figure}[H]
\begin{center}
\resizebox{0.4\textwidth}{!}
{
\begin{pspicture}(0,-1.008125)(5.9828124,1.008125)
\psline[linewidth=0.04cm](0.9809375,0.8096875)(4.9809375,0.8096875)
\psline[linewidth=0.04cm](0.9809375,-0.1903125)(4.9809375,-0.1903125)
\usefont{T1}{ptm}{m}{n}
\rput(0.41234374,0.8146875){$z=0$}
\usefont{T1}{ptm}{m}{n}
\rput(0.23234375,-0.1853125){$d$}
\usefont{T1}{ptm}{m}{n}
\rput(3.9423437,0.2146875){$\sigma_1d=\tau$}
\usefont{T1}{ptm}{m}{n}
\rput(4.302344,-0.7853125){$\sigma_2\ll \sigma_1$}
\end{pspicture} 
}
\caption{Model 5}
\label{fig:6-model5}
\end{center}
\end{figure}
$d\ll p_1$ for $|K_1|\gg |K_2| \Rightarrow$
\begin{align*}
G_1^-=\frac{K_2+K_1\tanh(K_1d)}{K_1}
\end{align*}
\begin{align*}
C(k,\omega)=\frac{1}{K_2+K_1\tanh(K_1d)}\stackrel{kp\rightarrow 0}\rightarrow \frac{1}{K_2+K_1^2d}=\frac{C_2}{1+i\omega\mu_0\tau C_2}
\end{align*}

with $C_2=K_2^{-1}=\frac{p_2}{1+i}$. 

Phase of $C$: $[-45^\circ,-90^\circ$]

Phase of $z$: $[45^\circ,0^\circ$]

\begin{figure}[H]
\begin{center}
\resizebox{0.6\textwidth}{!}
{
\begin{pspicture}(0,-3.3573437)(11.522813,3.3573437)
\psline[linewidth=0.04cm,arrowsize=0.05291667cm 2.0,arrowlength=1.4,arrowinset=0.4]{->}(1.7995313,2.760469)(1.7995313,-3.239531)
\psline[linewidth=0.04cm,arrowsize=0.05291667cm 2.0,arrowlength=1.4,arrowinset=0.4]{->}(1.7995313,2.760469)(9.799531,2.760469)
\usefont{T1}{ptm}{m}{n}
\rput(10.622344,3.0654688){$-Im(C_0)$}
\usefont{T1}{ptm}{m}{n}
\rput(0.76234376,-3.1345313){$Re(C_0)$}
\psline[linewidth=0.04cm](1.7995313,2.760469)(9.599531,-1.8395312)
\usefont{T1}{ptm}{m}{n}
\rput(9.849532,-1.0345311){Model 1}
\psline[linewidth=0.04cm,arrowsize=0.05291667cm 2.0,arrowlength=1.4,arrowinset=0.4]{->}(5.199531,0.56046885)(5.9995313,0.06046885)
\usefont{T1}{ptm}{m}{n}
\rput(6.162344,-0.13453116){$T$}
\psbezier[linewidth=0.04,linestyle=dashed,dash=0.16cm 0.16cm](1.76,0.6589062)(3.56,0.6589062)(6.56,0.55890626)(9.16,-2.5410938)
\usefont{T1}{ptm}{m}{n}
\rput(3.378594,-2.2345312){Model 2}
\psbezier[linewidth=0.04,linestyle=dashed,dash=0.16cm 0.16cm](6.56,2.7589064)(5.76,1.1589062)(6.36,0.25890625)(9.86,-1.3410938)
\usefont{T1}{ptm}{m}{n}
\rput(8.863593,0.9654688){Model 3}
\usefont{T1}{ptm}{m}{n}
\rput(6.711406,3.1639063){$1/\omega\mu_0\tau$}
\usefont{T1}{ptm}{m}{n}
\rput(1.4114063,0.6639063){$h$}
\end{pspicture} 
}
\caption{Real and Imaginary part of $C$ in dependency of $T$ for Model 4 and 5}
\label{fig:crealimag2}
\end{center}
\end{figure}


\input{sections/05_induction/lect10}

